Use machine integers

src/examples/matmul/GPU.MatMul.Pure.fsti
@@ -4,54 +4,55 @@ module GPU.MatMul.Pure
 
 open FStar.Mul
 open Pulse.Lib.Pervasives
+module U64 = FStar.UInt64
 
 let rec matmul_single
   (rows shared columns: nat)
-  (s1: erased (Seq.Base.seq int){ Seq.Base.length s1 == rows * shared })
-  (s2 : erased (Seq.Base.seq int){ Seq.Base.length s2 == shared * columns })
+  (s1: erased (Seq.Base.seq U64.t){ Seq.Base.length s1 == rows * shared })
+  (s2 : erased (Seq.Base.seq U64.t){ Seq.Base.length s2 == shared * columns })
   (row: erased nat{row < rows}) (col: erased nat{col < columns}) (to: nat)
-    : GTot (erased int) (decreases to)
+    : GTot (erased U64.t) (decreases to)
   =
-  if reveal to > shared then 0 else if reveal to = 0 then 0 else
+  if reveal to > shared then 0UL else if reveal to = 0 then 0UL else
     (
         assert ((row + 1) <= rows /\ (row + 1) * shared <= rows * shared);
-        Seq.Base.index s1 (row * shared + (to - 1)) * Seq.Base.index s2 (col + (to - 1) * columns) + (matmul_single rows shared columns s1 s2 row col (to - 1))
+        U64.add_mod (U64.mul_mod (Seq.Base.index s1 (row * shared + (to - 1))) (Seq.Base.index s2 (col + (to - 1) * columns))) (matmul_single rows shared columns s1 s2 row col (to - 1))
     )
 
 let matmul_single_lemma
   (rows shared columns: erased nat)
-  (s1: erased (Seq.Base.seq int){ Seq.Base.length s1 == rows * shared })
-  (s2 : erased (Seq.Base.seq int){ Seq.Base.length s2 == shared * columns })
+  (s1: erased (Seq.Base.seq U64.t){ Seq.Base.length s1 == rows * shared })
+  (s2 : erased (Seq.Base.seq U64.t){ Seq.Base.length s2 == shared * columns })
   (row: erased nat{row < rows}) (col: erased nat{col < columns}) (to: nat)
     : Lemma
       (requires (0 < to /\ to <= shared))
       (ensures (
         assert ((row + 1) <= rows /\ (row + 1) * shared <= rows * shared);
-        reveal (matmul_single rows shared columns s1 s2 row col to) = Seq.Base.index s1 (row * shared + (to - 1)) * Seq.Base.index s2 (col + (to - 1) * columns) + (matmul_single rows shared columns s1 s2 row col (to - 1))
+        reveal (matmul_single rows shared columns s1 s2 row col to) = U64.add_mod (U64.mul_mod (Seq.Base.index s1 (row * shared + (to - 1))) (Seq.Base.index s2 (col + (to - 1) * columns))) (matmul_single rows shared columns s1 s2 row col (to - 1))
       ))
   = ()
 
 private let matmul_single_at
   (rows shared columns: erased nat)
-  (s1: erased (Seq.Base.seq int){ Seq.Base.length s1 == rows * shared })
-  (s2 : erased (Seq.Base.seq int){ Seq.Base.length s2 == shared * columns })
+  (s1: erased (Seq.Base.seq U64.t){ Seq.Base.length s1 == rows * shared })
+  (s2 : erased (Seq.Base.seq U64.t){ Seq.Base.length s2 == shared * columns })
   (idx: nat{idx < rows * columns})
-    : GTot int
+    : GTot U64.t
   =
   let row = idx / columns in let col = idx % columns in matmul_single rows shared columns s1 s2 row col shared
 
 let matmul
   (rows shared columns: erased nat)
-  (s1: erased (Seq.Base.seq int){ Seq.Base.length s1 == rows * shared })
-  (s2 : erased (Seq.Base.seq int){ Seq.Base.length s2 == shared * columns })
-    : GTot (sr:(Seq.Base.seq int){ Seq.Base.length sr == rows * columns })
+  (s1: erased (Seq.Base.seq U64.t){ Seq.Base.length s1 == rows * shared })
+  (s2 : erased (Seq.Base.seq U64.t){ Seq.Base.length s2 == shared * columns })
+    : GTot (sr:(Seq.Base.seq U64.t){ Seq.Base.length sr == rows * columns })
   =
   Seq.Base.init_ghost (rows * columns) (matmul_single_at rows shared columns s1 s2)
 
 let lemma_matmul_index
   (rows shared columns: erased nat)
-  (s1: erased (Seq.Base.seq int){ Seq.Base.length s1 == rows * shared })
-  (s2 : erased (Seq.Base.seq int){ Seq.Base.length s2 == shared * columns })
+  (s1: erased (Seq.Base.seq U64.t){ Seq.Base.length s1 == rows * shared })
+  (s2 : erased (Seq.Base.seq U64.t){ Seq.Base.length s2 == shared * columns })
   (idx: nat{idx < rows * columns})
     : Lemma
       (ensures (Seq.Base.index (reveal (matmul rows shared columns s1 s2)) idx) == reveal (matmul_single rows shared columns s1 s2 (idx / columns) (idx % columns) shared))
