src/examples/matmul/GPU.MatMul.Kernel.fsti
@@ -9,14 +9,15 @@ open GPU
 module Impure = GPU.MatMul.Impure
 module Pure = GPU.MatMul.Pure
 module SZ = FStar.SizeT
+module U64 = FStar.UInt64
 
 let singleton #a (elem: a) : Seq.Base.seq a = Seq.Base.cons elem Seq.Base.empty
 
 let kpre_pair (rows shared columns: nat)
-  (ga1: gpu_array int (rows * shared))
-  (ga2: gpu_array int (shared * columns))
-  (#s1: erased (Seq.Base.seq int))
-  (#s2: erased (Seq.Base.seq int))
+  (ga1: gpu_array U64.t (rows * shared))
+  (ga2: gpu_array U64.t (shared * columns))
+  (#s1: erased (Seq.Base.seq U64.t))
+  (#s2: erased (Seq.Base.seq U64.t))
   (nth: erased nat { nth > 0 })
   : slprop
   =
@@ -24,11 +25,11 @@ let kpre_pair (rows shared columns: nat)
   ** Impure.gpu_pts_to_matrix shared columns ga2 nth s2
 
 let kpre (rows shared columns: nat)
-  (ga1: gpu_array int (rows * shared))
-  (ga2: gpu_array int (shared * columns))
-  (r: gpu_array int (rows * columns))
-  (#s1: erased (Seq.Base.seq int) )
-  (#s2: erased (Seq.Base.seq int))
+  (ga1: gpu_array U64.t (rows * shared))
+  (ga2: gpu_array U64.t (shared * columns))
+  (r: gpu_array U64.t (rows * columns))
+  (#s1: erased (Seq.Base.seq U64.t) )
+  (#s2: erased (Seq.Base.seq U64.t))
   (nth: erased nat { reveal nth == rows * columns })
   (tid : nat{ tid < rows * columns})
   : slprop
@@ -37,11 +38,11 @@ let kpre (rows shared columns: nat)
   ** (exists* sr. gpu_pts_to_array_slice r tid (tid+1) sr)
 
 let kpost (rows shared columns: nat)
-  (ga1: gpu_array int (rows * shared))
-  (ga2: gpu_array int (shared * columns))
-  (r: gpu_array int (rows * columns))
-  (#s1: erased (Seq.Base.seq int) {Seq.Base.length s1 == rows * shared})
-  (#s2: erased (Seq.Base.seq int) {Seq.Base.length s2 == shared * columns})
+  (ga1: gpu_array U64.t (rows * shared))
+  (ga2: gpu_array U64.t (shared * columns))
+  (r: gpu_array U64.t (rows * columns))
+  (#s1: erased (Seq.Base.seq U64.t) {Seq.Base.length s1 == rows * shared})
+  (#s2: erased (Seq.Base.seq U64.t) {Seq.Base.length s2 == shared * columns})
   (nth: erased nat { reveal nth == rows * columns })
   (tid : nat {  tid < rows * columns })
   : slprop
@@ -60,9 +61,9 @@ let columns : nat = 255 // columns of ga2/r
 ```pulse
 fn kernel
   // (rows: nat) (shared: nat { shared < pow2 16 }) (columns: nat)
-  (ga1 : gpu_array int (rows * shared)) (ga2 : gpu_array int (shared * columns)) (r : gpu_array int (rows * columns))
-  (#s1: erased (Seq.Base.seq int) {Seq.Base.length s1 == rows * shared})
-  (#s2: erased (Seq.Base.seq int) {Seq.Base.length s2 == shared * columns})
+  (ga1 : gpu_array U64.t (rows * shared)) (ga2 : gpu_array U64.t (shared * columns)) (r : gpu_array U64.t (rows * columns))
+  (#s1: erased (Seq.Base.seq U64.t) {Seq.Base.length s1 == rows * shared})
+  (#s2: erased (Seq.Base.seq U64.t) {Seq.Base.length s2 == shared * columns})
   (nth : erased nat { nth == rows * columns })
   (tid : nat{ tid < nth })
   requires gpu
@@ -79,7 +80,7 @@ fn kernel
   // assert (pure (0 <= trow /\ trow < rows /\ 0 <= tcol /\ tcol < columns));
 
   let mut i = 0sz;
-  let mut sum = 0;
+  let mut sum = 0UL;
 
   while (let v = !i; (SZ.v v < shared))
      invariant b.
@@ -88,23 +89,23 @@ fn kernel
        pts_to i v **
        gpu **
        pts_to sum (Pure.matmul_single rows shared columns s1 s2 trow tcol (SZ.v v))
-       ** Impure.gpu_pts_to_matrix rows shared ga1 nth s1
-       ** Impure.gpu_pts_to_matrix shared columns ga2 nth s2
+       ** Impure.gpu_pts_to_matrix #U64.t rows shared ga1 nth s1
+       ** Impure.gpu_pts_to_matrix #U64.t shared columns ga2 nth s2
   {
     let v = !i;
     let s = !sum;
-    let v1 = Impure.gpu_matrix_read #int #rows #shared ga1 #nth #s1 trow (SZ.v v);
-    let v2 = Impure.gpu_matrix_read #int #shared #columns ga2 #nth #s2 (SZ.v v) tcol;
+    let v1 = Impure.gpu_matrix_read #U64.t #rows #shared ga1 #nth #s1 trow (SZ.v v);
+    let v2 = Impure.gpu_matrix_read #U64.t #shared #columns ga2 #nth #s2 (SZ.v v) tcol;
 
     i := SZ.add v 1sz;
-    sum := s + (v1 * v2);
+    sum := U64.add_mod (U64.mul_mod v1 v2) s;
 
     (**)Pure.matmul_single_lemma rows shared columns s1 s2 trow tcol (SZ.v (SZ.add v 1sz));
     ()
   };
 
   let s = !sum;
-  gpu_array_write #int #_ #tid #(tid+1) r tid s;
+  gpu_array_write #U64.t #_ #tid #(tid+1) r tid s;
 
 
   with #v. assert (gpu_pts_to_array_slice r tid (tid + 1) v);
@@ -121,10 +122,10 @@ fn kernel
 ```pulse
 ghost fn fold_pre_pair
   (rows shared columns: nat)
-  (ga1: gpu_array int (rows * shared))
-  (ga2: gpu_array int (shared * columns))
-  (#s1: erased (Seq.Base.seq int) {Seq.Base.length s1 == rows * shared})
-  (#s2: erased (Seq.Base.seq int) {Seq.Base.length s2 == shared * columns})
+  (ga1: gpu_array U64.t (rows * shared))
+  (ga2: gpu_array U64.t (shared * columns))
+  (#s1: erased (Seq.Base.seq U64.t) {Seq.Base.length s1 == rows * shared})
+  (#s2: erased (Seq.Base.seq U64.t) {Seq.Base.length s2 == shared * columns})
   (nth: erased nat { nth > 0 })
   (tid: nat)
   requires Impure.gpu_pts_to_matrix rows shared ga1 nth s1
@@ -139,16 +140,16 @@ ghost fn fold_pre_pair
 ```pulse
 ghost fn fold_pre
   (rows shared columns: nat)
-  (ga1: gpu_array int (rows * shared))
-  (ga2: gpu_array int (shared * columns))
-  (gr: gpu_array int (rows * columns))
-  (#s1: erased (Seq.Base.seq int) {Seq.Base.length s1 == rows * shared})
-  (#s2: erased (Seq.Base.seq int) {Seq.Base.length s2 == shared * columns})
-  (#sr: (Seq.Base.seq int) {Seq.Base.length sr == 1})
+  (ga1: gpu_array U64.t (rows * shared))
+  (ga2: gpu_array U64.t (shared * columns))
+  (gr: gpu_array U64.t (rows * columns))
+  (#s1: erased (Seq.Base.seq U64.t) {Seq.Base.length s1 == rows * shared})
+  (#s2: erased (Seq.Base.seq U64.t) {Seq.Base.length s2 == shared * columns})
+  (#sr: (Seq.Base.seq U64.t) {Seq.Base.length sr == 1})
   (nth: erased nat { nth == (rows * columns) })
   (tid: nat { tid < nth /\ tid < rows * columns })
   requires kpre_pair rows shared columns ga1 ga2 #s1 #s2 nth
-        ** gpu_pts_to_array_slice #int #nth gr tid (tid+1) sr
+        ** gpu_pts_to_array_slice #U64.t #nth gr tid (tid+1) sr
   ensures  kpre rows shared columns ga1 ga2 gr #s1 #s2 nth tid
 {
   fold kpre rows shared columns ga1 ga2 gr #s1 #s2 nth tid;
@@ -162,11 +163,11 @@ ghost fn fold_pre
 ```pulse
 ghost fn unfold_post
   (rows shared columns: nat)
-  (ga1: gpu_array int (rows * shared))
-  (ga2: gpu_array int (shared * columns))
-  (gr: gpu_array int (rows * columns))
-  (#s1: erased (Seq.Base.seq int) {Seq.Base.length s1 == rows * shared})
-  (#s2: erased (Seq.Base.seq int) {Seq.Base.length s2 == shared * columns})
+  (ga1: gpu_array U64.t (rows * shared))
+  (ga2: gpu_array U64.t (shared * columns))
+  (gr: gpu_array U64.t (rows * columns))
+  (#s1: erased (Seq.Base.seq U64.t) {Seq.Base.length s1 == rows * shared})
+  (#s2: erased (Seq.Base.seq U64.t) {Seq.Base.length s2 == shared * columns})
   (nth: erased nat { reveal nth == rows * columns })
   (tid: nat {  tid < rows * columns })
   requires kpost rows shared columns ga1 ga2 gr #s1 #s2 nth tid
